Util.v
@@ -3,6 +3,9 @@ Unset Strict Implicit.
 Unset Printing Implicit Defensive. 
 Generalizable All Variables.
 
+Require Import List.
+Require Import Program.
+
 Class Apply a b c := 
   {
     apply : a -> b -> c
@@ -10,6 +13,8 @@ Class Apply a b c :=
 
 Infix "$" := apply (at level 85, right associativity) : prog_scope.
 Infix "$$" := apply (at level 15, left associativity) : prog_scope.
+Infix "<<" := compose (at level 40) : prog_scope.
+Infix ">>" := (flip compose) (at level 40) : prog_scope.
 
 Definition apply_arrow {A B} (f : A -> B) x := f x.
 
@@ -21,5 +26,15 @@ Instance Apply_arrow A B : Apply (A -> B) A B :=
 Class Max t := 
   {
     max : t -> t -> t
+  }.
+
+Class Find key value container := 
+  {
+    find : key -> container -> option value
+  }.
+
+Instance Find_list A : Find nat A (list A) :=
+  {
+    find k c := @nth_error A c k
   }.
 
