EBool.v
@@ -1,0 +1,49 @@
+Require Import Util.
+Require Import TypingFacts.
+
+Export Typing.
+
+Local Open Scope prog_scope.
+
+Definition Tbool := Tsum Tunit Tunit.
+Definition Etrue := Einl $$ Tunit $$ Tunit $$ Ett.
+Definition Efalse := Einr $$ Tunit $$ Tunit $$ Ett.
+Definition Eif e b_true b_false :=
+  Ematch_sum e (shift b_true) (shift b_false).
+
+Lemma Kbool T : kinding T Tbool 0.
+Proof.
+  eapply Ksum'; eapply Kunit.
+Qed.
+
+Definition bool_size := Sinlinr Stt Stt.
+
+Local Open Scope F.
+
+Lemma TPif T e e1 e2 n s' t n1 n2 s s1 s2 :
+  typing T e Tbool n s' ->
+  is_inlinr s' = Some (s1, s2) ->
+  typing T e1 t n1 s ->
+  typing T e2 t n2 s ->
+  typing T (Eif e e1 e2) t (n + F1 + max n1 n2) s.
+Proof.
+  intros He Hs H1 H2.
+  {
+    eapply TPsubn.
+    {
+      eapply TPmatch_inlinr.
+      { eauto. }
+      { eauto. }
+      { eapply TPinsert0; eauto. }
+      { eapply TPinsert0; eauto. }
+    }
+    {
+      simpl.
+      repeat rewrite fold_subst_s_f.
+      repeat rewrite fold_shift_from_f.
+      repeat rewrite subst_shift_s_f.
+      reflexivity.
+    }
+  }
+Qed.
+
