TypeSoundness.v
@@ -1,0 +1,58 @@
+(* Type soundness *)
+
+Require Import List.
+Require Import Typing EvalCBV.
+
+Import ListNotations.
+Local Open Scope list_scope.
+
+(* encoding of fix by recursive-type :
+     fix f(x).e := \y. (unfold v) v y 
+        where v := fold (\z. (\f. \x. e) (\y. (unfold z) z y)) 
+                    (for y,z\not\in FV(e))
+ *)
+
+Inductive nsteps : expr -> nat -> expr -> Prop :=
+| Nsteps0 e : nsteps e 0 e
+| NstepsS e1 e2 n e3 : step e1 e2 -> nsteps e2 n e3 -> nsteps e1 (S n) e3
+.
+
+Inductive steps : expr -> expr -> Prop :=
+| Steps0 e : steps e e
+| StepsS e1 e2 e3 : step e1 e2 -> steps e2 e3 -> steps e1 e3
+.
+
+Definition get_size (e : expr) : size.
+  admit.
+Defined.
+
+Definition typingsim T e t := exists c s, typing T e t c s.
+
+Local Open Scope G.
+
+Definition nat_of_cexpr (c : cexpr) : option nat.
+  admit.
+Defined.
+
+Definition nostuck e := forall e', steps e e' -> IsValue e' \/ exists e'', step e' e''.
+
+Theorem type_soundness : forall t1 c s e t, 
+  typing [TEtyping (t1, None)] e t c s -> 
+  (forall v1,
+     IsValue v1 ->
+     typingsim [] v1 t1 ->
+     nostuck (subst v1 e)) /\
+  exists Ct s0, 
+    forall v1,
+      IsValue v1 ->
+      typingsim [] v1 t1 ->
+      let s1 := get_size v1 in
+      (s0 <= s1) ->
+      forall v n, 
+        IsValue v -> 
+        nsteps (subst v1 e) n v ->
+        (exists c_s1, nat_of_cexpr (subst s1 c) = Some c_s1 /\ n <= Ct * c_s1) /\
+        get_size v <= subst s1 s.
+Proof.
+  admit.
+Qed.
