Util2.v
@@ -1,0 +1,56 @@
+Set Implicit Arguments.
+
+Require Import List.
+Require Import Program.
+Require Import Util.
+
+Import ListNotations.
+Local Open Scope list_scope.
+
+Fixpoint range begin len :=
+  match len with
+    | 0 => nil
+    | S n => begin :: range (S begin) n
+  end.
+
+Definition assoc_list A B := list (A * B).
+
+Class Functor F :=
+  {
+    map : forall A B, (A -> B) -> F A -> F B
+  }.
+
+Instance Functor_list : Functor list :=
+  {
+    map := List.map
+  }.
+
+Instance Functor_option : Functor option :=
+  {
+    map := option_map
+  }.
+
+Definition map_snd {A B C} (f : B -> C) (p : A * B) := (fst p, f (snd p)).
+
+Definition map_assoc_list A B C (f : B -> C) (ls : assoc_list A B) := map (map_snd f) ls.
+
+Instance Functor_assoc_list A : Functor (assoc_list A) :=
+  {
+    map := @map_assoc_list A
+  }.
+
+Arguments rev {A} _.
+
+Definition cat_options {A} (ls : list (option A)) := fold_right (fun x acc => match x with Some v => v :: acc | _ => acc end) [] ls.
+
+Local Open Scope prog_scope.
+
+Definition map_option {A B} (f : A -> option B) := cat_options << map f.
+
+Fixpoint repeat A (a : A) n :=
+  match n with
+    | O => nil
+    | S n => a :: repeat a n
+  end.
+
+Definition removen A n ls := @firstn A n ls ++ skipn (S n) ls.
